SSA/Experimental/Bits/Fast/Reflect.lean
@@ -123,20 +123,24 @@ def Term.quote (t : _root_.Term) : Expr :=
   | shiftL t₁ n => mkApp2 (mkConst ``Term.shiftL) (t₁.quote) (mkNatLit n)
 
 open Lean in
+def mkConstBin (atp : Name) : Expr :=
+  mkApp (mkConst ``Predicate.binary) (mkConst atp)
+
+open Lean in
 def Predicate.quote (p : _root_.Predicate) : Expr :=
   match p with
-  | widthEq n => mkApp (mkConst ``Predicate.widthEq) (mkNatLit n)
-  | widthNeq n => mkApp (mkConst ``Predicate.widthNeq) (mkNatLit n)
-  | widthLt n => mkApp (mkConst ``Predicate.widthLt) (mkNatLit n)
-  | widthLe n => mkApp (mkConst ``Predicate.widthLe) (mkNatLit n)
-  | widthGt n => mkApp (mkConst ``Predicate.widthGt) (mkNatLit n)
-  | widthGe n => mkApp (mkConst ``Predicate.widthGe) (mkNatLit n)
-  | eq a b => mkApp2 (mkConst ``Predicate.eq) (_root_.Term.quote a) (_root_.Term.quote b)
-  | neq a b => mkApp2 (mkConst ``Predicate.neq) (_root_.Term.quote a) (_root_.Term.quote b)
-  | ult a b => mkApp2 (mkConst ``Predicate.ult) (_root_.Term.quote a) (_root_.Term.quote b)
-  | ule a b => mkApp2 (mkConst ``Predicate.ule) (_root_.Term.quote a) (_root_.Term.quote b)
-  | slt a b => mkApp2 (mkConst ``Predicate.slt) (_root_.Term.quote a) (_root_.Term.quote b)
-  | sle a b => mkApp2 (mkConst ``Predicate.sle) (_root_.Term.quote a) (_root_.Term.quote b)
+  | .width .eq n => mkApp2 (mkConst ``Predicate.width) (mkConst ``WidthPredicate.eq) (mkNatLit n)
+  | .width .neq n => mkApp2 (mkConst ``Predicate.width) (mkConst ``WidthPredicate.neq) (mkNatLit n)
+  | .width .lt n => mkApp2 (mkConst ``Predicate.width) (mkConst ``WidthPredicate.lt) (mkNatLit n)
+  | .width .le n => mkApp2 (mkConst ``Predicate.width) (mkConst ``WidthPredicate.le) (mkNatLit n)
+  | .width .gt n => mkApp2 (mkConst ``Predicate.width) (mkConst ``WidthPredicate.gt) (mkNatLit n)
+  | .width .ge n => mkApp2 (mkConst ``Predicate.width) (mkConst ``WidthPredicate.ge) (mkNatLit n)
+  | .binary .eq a b => mkApp2 (mkConstBin ``BinaryPredicate.eq) (_root_.Term.quote a) (_root_.Term.quote b)
+  | .binary .neq a b => mkApp2 (mkConstBin ``BinaryPredicate.neq) (_root_.Term.quote a) (_root_.Term.quote b)
+  | .binary .ult a b => mkApp2 (mkConstBin ``BinaryPredicate.ult) (_root_.Term.quote a) (_root_.Term.quote b)
+  | .binary .ule a b => mkApp2 (mkConstBin ``BinaryPredicate.ule) (_root_.Term.quote a) (_root_.Term.quote b)
+  | .binary .slt a b => mkApp2 (mkConstBin ``BinaryPredicate.slt) (_root_.Term.quote a) (_root_.Term.quote b)
+  | .binary .sle a b => mkApp2 (mkConstBin ``BinaryPredicate.sle) (_root_.Term.quote a) (_root_.Term.quote b)
   | land p q => mkApp2 (mkConst ``Predicate.land) (Predicate.quote p) (Predicate.quote q)
   | lor p q => mkApp2 (mkConst ``Predicate.lor) (Predicate.quote p) (Predicate.quote q)
 
@@ -368,20 +372,20 @@ theorem Term.denote_eq_eval_land_lt (t : Term) {w : Nat} {vars : List (BitVec w)
 
 def Predicate.denote (p : Predicate) (w : Nat) (vars : List (BitVec w)) : Prop :=
   match p with
-  | .widthGe k => k ≤ w -- w ≥ k
-  | .widthGt k => k < w -- w > k
-  | .widthLe k => w ≤ k
-  | .widthLt k => w < k
-  | .widthNeq k => w ≠ k
-  | .widthEq k => w = k
-  | .eq t₁ t₂ => t₁.denote w vars = t₂.denote w vars
-  | .neq t₁ t₂ => t₁.denote w vars ≠ t₂.denote w vars
+  | .width .ge k => k ≤ w -- w ≥ k
+  | .width .gt k => k < w -- w > k
+  | .width .le k => w ≤ k
+  | .width .lt k => w < k
+  | .width .neq k => w ≠ k
+  | .width .eq k => w = k
+  | .binary .eq t₁ t₂ => t₁.denote w vars = t₂.denote w vars
+  | .binary .neq t₁ t₂ => t₁.denote w vars ≠ t₂.denote w vars
   | .land  p q => p.denote w vars ∧ q.denote w vars
   | .lor  p q => p.denote w vars ∨ q.denote w vars
-  | .sle  t₁ t₂ => ((t₁.denote w vars).sle (t₂.denote w vars)) = true
-  | .slt  t₁ t₂ => ((t₁.denote w vars).slt (t₂.denote w vars)) = true
-  | .ule  t₁ t₂ => ((t₁.denote w vars) ≤ (t₂.denote w vars))
-  | .ult  t₁ t₂ => (t₁.denote w vars) < (t₂.denote w vars)
+  | .binary .sle  t₁ t₂ => ((t₁.denote w vars).sle (t₂.denote w vars)) = true
+  | .binary .slt  t₁ t₂ => ((t₁.denote w vars).slt (t₂.denote w vars)) = true
+  | .binary .ule  t₁ t₂ => ((t₁.denote w vars) ≤ (t₂.denote w vars))
+  | .binary .ult  t₁ t₂ => (t₁.denote w vars) < (t₂.denote w vars)
 
 /--
 The cost model of the predicate, which is based on the cardinality of the state space,
@@ -617,57 +621,51 @@ The predicate, when evaluated, at index `i` is false iff the denotation is true.
 theorem Predicate.eval_eq_denote (w : Nat) (p : Predicate) (vars : List (BitVec w)) :
     (p.eval (vars.map BitStream.ofBitVec) w = false) ↔ p.denote w vars := by
   induction p generalizing vars w
-  case widthEq n => simp [eval, denote]
-  case widthNeq n => simp [eval, denote]
-  case widthLt n => simp [eval, denote]
-  case widthLe n => simp [eval, denote]
-  case widthGt n => simp [eval, denote]
-  case widthGe n => simp [eval, denote]
-  case eq a b => simp [eval, denote]; apply evalEq_denote_false_iff
-  case neq a b => simp [eval, denote]; apply evalNeq_denote
-  case ult a b => simp [eval, denote]; apply evalUlt_denote_false_iff
-  case slt a b =>
-    simp [eval, denote];
-    by_cases h : Term.denote w a vars <ₛ Term.denote w b vars
-    · rw [h]
-      simp [Predicate.evalSlt_denote_false_iff, h]
-    · simp at h
-      rw [h]
-      simp only [Bool.not_false]
-      by_contra h'
-      simp only [Bool.not_eq_true] at h'
-      rw [Predicate.evalSlt_denote_false_iff] at h'
-      simp only [h, Bool.false_eq_true] at h'
-  case ule a b =>
-    simp [eval, denote];
-    simp only [evalLor, BitStream.and_eq]
-    rw [BitVec.ForLean.ule_iff_ult_or_eq]
-    by_cases heq : Term.denote w a vars = Term.denote w b vars
-    · rw [heq]
-      simp [evalEq_denote_false_iff a b vars |>.mpr heq]
-    · simp [heq]
-      by_cases hlt : Term.denote w a vars < Term.denote w b vars
-      · simp [hlt]
-        simp [evalUlt_denote_false_iff a b vars |>.mpr hlt]
-      · simp [hlt]
-        have := evalEq_denote_false_iff a b vars |>.not |>.mpr heq
-        simp only [this, true_and]
-        have := evalUlt_denote_false_iff a b vars |>.not |>.mpr hlt
-        simp only [this]
-  case sle a b =>
-    simp [eval, denote]
-    simp only [evalLor, BitStream.and_eq]
-    have h := BitVec.sle_iff_slt_or_eq (Term.denote w a vars) (Term.denote w b vars) |>.eq
-    rcases hSle : Term.denote w a vars ≤ₛ Term.denote w b vars
-    · simp [hSle] at h ⊢
-      obtain ⟨h₁, h₂⟩ := h
-      simp [evalEq_denote_true_iff .. |>.mpr h₁]
-      rw [evalSlt_denote_true_iff .. |>.mpr]
-      simp [h₂]
-    · simp [hSle] at h ⊢
-      intros hEq
-      simp [evalEq_denote_true_iff .. |>.mp hEq] at h
-      apply evalSlt_denote_false_iff .. |>.mpr h
+  case width rel _ => rcases rel <;> simp [eval, denote]
+  case binary rel a b =>
+    rcases rel
+    · simp [eval, denote]; apply evalEq_denote_false_iff
+    · simp [eval, denote]; apply evalNeq_denote
+    · simp [eval, denote]; apply evalUlt_denote_false_iff
+    · simp [eval, denote];
+      simp only [evalLor, BitStream.and_eq]
+      rw [BitVec.ForLean.ule_iff_ult_or_eq]
+      by_cases heq : Term.denote w a vars = Term.denote w b vars
+      · rw [heq]
+        simp [evalEq_denote_false_iff a b vars |>.mpr heq]
+      · simp [heq]
+        by_cases hlt : Term.denote w a vars < Term.denote w b vars
+        · simp [hlt]
+          simp [evalUlt_denote_false_iff a b vars |>.mpr hlt]
+        · simp [hlt]
+          have := evalEq_denote_false_iff a b vars |>.not |>.mpr heq
+          simp only [this, true_and]
+          have := evalUlt_denote_false_iff a b vars |>.not |>.mpr hlt
+          simp only [this]
+    · simp [eval, denote];
+      by_cases h : Term.denote w a vars <ₛ Term.denote w b vars
+      · rw [h]
+        simp [Predicate.evalSlt_denote_false_iff, h]
+      · simp at h
+        rw [h]
+        simp only [Bool.not_false]
+        by_contra h'
+        simp only [Bool.not_eq_true] at h'
+        rw [Predicate.evalSlt_denote_false_iff] at h'
+        simp only [h, Bool.false_eq_true] at h'
+    · simp [eval, denote]
+      simp only [evalLor, BitStream.and_eq]
+      have h := BitVec.sle_iff_slt_or_eq (Term.denote w a vars) (Term.denote w b vars) |>.eq
+      rcases hSle : Term.denote w a vars ≤ₛ Term.denote w b vars
+      · simp [hSle] at h ⊢
+        obtain ⟨h₁, h₂⟩ := h
+        simp [evalEq_denote_true_iff .. |>.mpr h₁]
+        rw [evalSlt_denote_true_iff .. |>.mpr]
+        simp [h₂]
+      · simp [hSle] at h ⊢
+        intros hEq
+        simp [evalEq_denote_true_iff .. |>.mp hEq] at h
+        apply evalSlt_denote_false_iff .. |>.mpr h
   case land p q hp hq => simp [eval, denote, hp, hq, evalLand]
   case lor p q hp hq =>
     simp [eval, denote, hp, hq]
@@ -973,11 +971,16 @@ TODO(@bollu): We also assume that the goals are in negation normal form, and if 
 namespace Reflect
 open Lean Meta Elab Tactic
 
+inductive AutomataBackend
+| fast
+-- | classic
+deriving Repr, DecidableEq
+
 inductive CircuitBackend
 /-- Pure lean implementation, verified. -/
-| lean 
+| lean (automata : AutomataBackend)
 /-- bv_decide based backend. Currently unverified. -/
-| cadical 
+| cadical
 /-- Dry run, do not execute and close proof with `sorry` -/
 | dryrun
 deriving Repr, DecidableEq
@@ -1003,7 +1006,7 @@ structure Config where
   /--
   Whether the tactic should use the (currently unverified) bv_decide based backend for solving constraints.
   -/
-  backend : CircuitBackend := .lean
+  backend : CircuitBackend := .lean .fast
 
 /-- Default user configuration -/
 def Config.default : Config := {}
@@ -1236,13 +1239,13 @@ partial def reflectPredicateAux (bvToIxMap : ReflectMap) (e : Expr) (wExpected :
         throwError "Only Nat expressions allowed are '{wExpected} ≠ <concrete value>'. Found {indentD e}."
       let some natVal ← Lean.Meta.getNatValue? b
         | throwError "Expected '{wExpected} ≠ <concrete width>', found symbolic width {indentD b}."
-      let out := Predicate.widthEq natVal
+      let out := Predicate.width .eq natVal
       return { bvToIxMap := bvToIxMap, e := out }
 
     | BitVec w =>
       let a ←  reflectTermUnchecked bvToIxMap w a
       let b ← reflectTermUnchecked a.bvToIxMap w b
-      return { bvToIxMap := b.bvToIxMap, e := Predicate.eq a.e b.e }
+      return { bvToIxMap := b.bvToIxMap, e := Predicate.binary .eq a.e b.e }
     | Bool =>
       -- Sadly, recall that slt, sle are of type 'BitVec w → BitVec w → Bool',
       -- so we get goal states of them form 'a <ₛb = true'.
@@ -1254,11 +1257,11 @@ partial def reflectPredicateAux (bvToIxMap : ReflectMap) (e : Expr) (wExpected :
       | BitVec.slt w a b =>
         let a ← reflectTermUnchecked bvToIxMap w a
         let b ← reflectTermUnchecked a.bvToIxMap w b
-        return { bvToIxMap := b.bvToIxMap, e := Predicate.slt a.e b.e }
+        return { bvToIxMap := b.bvToIxMap, e := Predicate.binary .slt a.e b.e }
       | BitVec.sle w a b =>
         let a ← reflectTermUnchecked bvToIxMap w a
         let b ← reflectTermUnchecked a.bvToIxMap w b
-        return { bvToIxMap := b.bvToIxMap, e := Predicate.sle a.e b.e }
+        return { bvToIxMap := b.bvToIxMap, e := Predicate.binary .sle a.e b.e }
       | _ =>
         throwError "unknown boolean conditional, expected 'bv.slt bv = true' or 'bv.sle bv = true'. Found {indentD e}"
     | _ =>
@@ -1272,24 +1275,24 @@ partial def reflectPredicateAux (bvToIxMap : ReflectMap) (e : Expr) (wExpected :
         throwError "Only Nat expressions allowed are '{wExpected} ≠ <concrete value>'. Found {indentD e}."
       let some natVal ← Lean.Meta.getNatValue? b
         | throwError "Expected '{wExpected} ≠ <concrete width>', found symbolic width {indentD b}."
-      let out := Predicate.widthNeq natVal
+      let out := Predicate.width .neq natVal
       return { bvToIxMap := bvToIxMap, e := out }
     | BitVec w =>
       let a ← reflectTermUnchecked bvToIxMap w a
       let b ← reflectTermUnchecked a.bvToIxMap w b
-      return { bvToIxMap := b.bvToIxMap, e := Predicate.neq a.e b.e }
+      return { bvToIxMap := b.bvToIxMap, e := Predicate.binary .neq a.e b.e }
     | _ =>
       throwError "Expected typeclass to be 'BitVec w' / 'Nat', found '{indentD α}' in {e} when matching against 'Ne'"
   | LT.lt α _inst a b =>
     let_expr BitVec w := α | throwError "Expected typeclass to be BitVec w, found '{indentD α}' in {indentD e} when matching against 'LT.lt'"
     let a ← reflectTermUnchecked bvToIxMap w a
     let b ← reflectTermUnchecked a.bvToIxMap w b
-    return { bvToIxMap := b.bvToIxMap, e := Predicate.ult a.e b.e }
+    return { bvToIxMap := b.bvToIxMap, e := Predicate.binary .ult a.e b.e }
   | LE.le α _inst a b =>
     let_expr BitVec w := α | throwError "Expected typeclass to be BitVec w, found '{indentD α}' in {indentD e} when matching against 'LE.le'"
     let a ← reflectTermUnchecked bvToIxMap w a
     let b ← reflectTermUnchecked a.bvToIxMap w b
-    return { bvToIxMap := b.bvToIxMap, e := Predicate.ule a.e b.e }
+    return { bvToIxMap := b.bvToIxMap, e := Predicate.binary .ule a.e b.e }
   | Or p q =>
     let p ← reflectPredicateAux bvToIxMap p wExpected
     let q ← reflectPredicateAux p.bvToIxMap q wExpected
@@ -1514,6 +1517,7 @@ partial def decideIfZerosAuxTermElabM {arity : Type _} [DecidableEq arity] [Fint
     let tElapsedSec := (tEnd - tStart) / 1000
     if h : le then 
       IO.eprintln s!"Inductive invariant established! (time={tElapsedSec}s)"
+    if h : le then
       return true
     else
       -- have _wf : card_compl (cNext ||| c) < card_compl c :=
@@ -1600,7 +1604,7 @@ def reflectUniversalWidthBVs (g : MVarId) (cfg : Config) : TermElabM (List MVarI
     let fsm := predicateEvalEqFSM result.e |>.toFSM
     logInfo f!"{fsm.format}'"
 
-    match cfg.backend with 
+    match cfg.backend with
     | .dryrun =>
         g.assign (← mkSorry (← g.getType) (synthetic := false))
         logInfo "Closing goal with 'sorry' for dry-run"
@@ -1617,7 +1621,7 @@ def reflectUniversalWidthBVs (g : MVarId) (cfg : Config) : TermElabM (List MVarI
       else
         throwError "failed to prove goal, since decideIfZerosM established that theorem is not true."
         return [g]
-    | .lean =>
+    | .lean .fast =>
       if fsm.circuitSize > cfg.circuitSizeThreshold then
         throwError "Not running on goal: since circuit size ('{fsm.circuitSize}') is larger than threshold ('circuitSizeThreshold:{cfg.circuitSizeThreshold}')"
       if fsm.stateSpaceSize > cfg.stateSpaceSizeThreshold then
@@ -1673,5 +1677,376 @@ def evalBvAutomataCircuit : Tactic := fun
       evalDecideCore `bv_automata_circuit (cfg := { native := true : Parser.Tactic.DecideConfig })
     | _gs => throwError "expected single goal after reflecting, found multiple goals. quitting"
 | _ => throwUnsupportedSyntax
+
+/-- Can solve explicitly quantified expressions with intros. bv_automata3. -/
+theorem eq1 : ∀ (w : Nat) (a : BitVec w), a = a := by
+  intros
+  bv_automata_circuit
+#print eq1
+
+/-- Can solve implicitly quantified expressions by directly invoking bv_automata3. -/
+theorem eq2 (w : Nat) (a : BitVec w) : a = a := by
+  bv_automata_circuit
+#print eq1
+
+open NNF in
+
+example (w : Nat) (a b : BitVec w) : a + b = b + a := by
+  bv_automata_circuit
+
+example (w : Nat) (a b : BitVec w) : (a + b = b + a) ∨ (a = 0#w) := by
+  bv_automata_circuit
+
+example (w : Nat) (a b : BitVec w) : (a = 0#w) ∨ (a + b = b + a) := by
+  bv_automata_circuit
+
+example (w : Nat) (a : BitVec w) : (a = 0#w) ∨ (a ≠ 0#w) := by
+  bv_automata_circuit
+
+example (w : Nat) (a b : BitVec w) : (a + b = b + a) ∧ (a + 0#w = a) := by
+  bv_automata_circuit
+
+example (w : Nat) (a b : BitVec w) : (a + 0#w = a) := by
+  bv_automata_circuit
+
+example (w : Nat) (a b : BitVec w) : (a + b = b + a) ∧ (a + 0#w = a) := by
+  bv_automata_circuit
+
+example (w : Nat) (a b : BitVec w) : (a ≠ b) → (b ≠ a) := by
+  bv_automata_circuit
+
+/-- either a < b or b ≤ a -/
+example (w : Nat) (a b : BitVec w) : (a < b) ∨ (b ≤ a) := by
+  bv_automata_circuit
+
+/-- Tricohotomy of < -/
+example (w : Nat) (a b : BitVec w) : (a < b) ∨ (b < a) ∨ (a = b) := by
+  bv_automata_circuit
+
+/-- < implies not equals -/
+example (w : Nat) (a b : BitVec w) : (a < b) → (a ≠ b) := by
+  bv_automata_circuit
+
+/-- <= and >= implies equals -/
+example (w : Nat) (a b : BitVec w) : ((a ≤ b) ∧ (b ≤ a)) → (a = b) := by
+  bv_automata_circuit
+
+example (a b : BitVec 1) : (a - b).slt 0 → a.slt b := by
+  fail_if_success bv_decide
+  -- The prover found a counterexample, consider the following assignment:
+  -- a = 0x0#1
+  -- b = 0x1#1
+  sorry
+
+-- This should succeed.
+example (w : Nat) (a b : BitVec w) : (w > 1 ∧ (a - b).slt 0 → a.slt b) := by
+  try bv_automata_circuit;
+  sorry
+
+
+/-- Tricohotomy of slt. Currently fails! -/
+example (w : Nat) (a b : BitVec w) : (a.slt b) ∨ (b.sle a) := by
+  bv_automata_circuit
+  -- TODO: I don't understand this metaprogramming error, I must be building the term weirdly...
+
+/-- Tricohotomy of slt. Currently fails! -/
+example (w : Nat) (a b : BitVec w) : (a.slt b) ∨ (b.slt a) ∨ (a = b) := by
+  bv_automata_circuit
+  -- TODO: I don't understand this metaprogramming error, I must be building the term weirdly...
+
+/-- a <=s b and b <=s a implies a = b-/
+example (w : Nat) (a b : BitVec w) : ((a.sle b) ∧ (b.sle a)) → a = b := by
+  bv_automata_circuit
+  -- TODO: I don't understand this metaprogramming error, I must be building the term weirdly...
+
+/-- In bitwidth 0, all values are equal.
+In bitwidth 1, 1 + 1 = 0.
+In bitwidth 2, 1 + 1 = 2 ≠ 0#2
+For all bitwidths ≥ 2, we know that a ≠ a + 1
+-/
+example (w : Nat) (a : BitVec w) : (a ≠ a + 1#w) ∨ (1#w + 1#w = 0#w) ∨ (1#w = 0#w):= by
+  bv_automata_circuit
+
+/-- If we have that 'a &&& a = 0`, then we know that `a = 0` -/
+example (w : Nat) (a : BitVec w) : (a &&& a = 0#w) → a = 0#w := by
+  bv_automata_circuit
+
+/--
+Is this true at bitwidth 1? Not it is not!
+So we need an extra hypothesis that rules out bitwifth 1.
+We do this by saying that either the given condition, or 1+1 = 0.
+I'm actually not sure why I need to rule out bitwidth 0? Mysterious!
+-/
+example (w : Nat) (a : BitVec w) : (w = 2) → ((a = - a) → a = 0#w) := by
+  fail_if_success bv_automata_circuit
+  sorry
+
+
+example (w : Nat) (a : BitVec w) : (w = 1) → (a = 0#w ∨ a = 1#w) := by bv_automata_circuit
+example (w : Nat) (a : BitVec w) : (w = 0) → (a = 0#w ∨ a = 1#w) := by bv_automata_circuit
+example (w : Nat) : (w = 1) → (1#w + 1#w = 0#w) := by bv_automata_circuit
+example (w : Nat) : (w = 0) → (1#w + 1#w = 0#w) := by bv_automata_circuit
+example (w : Nat) : ((w = 0) ∨ (w = 1)) → (1#w + 1#w = 0#w) := by bv_automata_circuit
+
+example (w : Nat) : (1#w + 1#w = 0#w) → ((w = 0) ∨ (w = 1)):= by
+  bv_automata_circuit
+/-
+We can say that we are at bitwidth 1 by saying that 1 + 1 = 0.
+When we have this, we then explicitly enumerate the different values that a can have.
+Note that this is pretty expensive.
+-/
+example (w : Nat) (a : BitVec w) : (1#w + 1#w = 0#w) → (a = 0#w ∨ a = 1#w) := by
+  bv_automata_circuit
+
+example (w : Nat) (a b : BitVec w) : (a + b = 0#w) → a = - b := by
+  bv_automata_circuit
+
+
+/-- Can use implications -/
+theorem eq_circuit (w : Nat) (a b : BitVec w) : (a &&& b = 0#w) → ((a + b) = (a ||| b)) := by
+  bv_nnf
+  bv_automata_circuit
+
+#print eq_circuit
+
+
+/-- Can exploit hyps -/
+theorem eq4 (w : Nat) (a b : BitVec w) (h : a &&& b = 0#w) : a + b = a ||| b := by
+  bv_automata_circuit
+
+#print eq_circuit
+
+section BvAutomataTests
+
+/-!
+# Test Cases
+-/
+
+/--
+warning: Tactic has not understood the following expressions, and will treat them as symbolic:
+
+  - 'f x'
+  - 'f y'
+-/
+#guard_msgs (warning, drop error, drop info) in
+theorem test_symbolic_abstraction (f : BitVec w → BitVec w) (x y : BitVec w) : f x ≠ f y :=
+  by bv_automata_circuit
+
+/-- Check that we correctly handle `OfNat.ofNat 1`. -/
+theorem not_neg_eq_sub_one (x : BitVec 53) :
+    ~~~ (- x) = x - 1 := by
+  bv_automata_circuit
+
+/-- Check that we correctly handle multiplication by two. -/
+theorem sub_eq_mul_and_not_sub_xor (x y : BitVec w):
+    x - y = 2 * (x &&& ~~~ y) - (x ^^^ y) := by
+  -- simp [Simplifications.BitVec.OfNat_ofNat_mul_eq_ofNat_mul]
+  -- simp only [BitVec.ofNat_eq_ofNat, Simplifications.BitVec.two_mul_eq_add_add]
+  all_goals bv_automata_circuit (config := {circuitSizeThreshold := 140 })
+
+
+/- See that such problems have large circuit sizes, but small state spaces -/
+def alive_1 {w : ℕ} (x x_1 x_2 : BitVec w) : (x_2 &&& x_1 ^^^ x_1) + 1#w + x = x - (x_2 ||| ~~~x_1) := by
+  bv_automata_circuit (config := { circuitSizeThreshold := 107 })
+
+
+def false_statement {w : ℕ} (x y : BitVec w) : x = y := by
+  fail_if_success bv_automata_circuit
+  sorry
+
+def test_OfNat_ofNat (x : BitVec 1) : 1#1 + x = x + 1#1 := by
+  bv_automata_circuit -- can't decide things for fixed bitwidth.
+
+def test0 {w : Nat} (x y : BitVec w) : x + 0#w = x := by
+  bv_automata_circuit
+
+
+def test_simple2 {w : Nat} (x y : BitVec w) : x = x := by
+  bv_automata_circuit
+
+def test1 {w : Nat} (x y : BitVec w) : (x ||| y) - (x ^^^ y) = x &&& y := by
+  bv_automata_circuit
+
+
+def test4 (x y : BitVec w) : (x + -y) = (x - y) := by
+  bv_automata_circuit
+
+def test5 (x y z : BitVec w) : (x + y + z) = (z + y + x) := by
+  bv_automata_circuit
+
+
+def test6 (x y z : BitVec w) : (x + (y + z)) = (x + y + z) := by
+  bv_automata_circuit
+
+def test11 (x y : BitVec w) : (x + y) = ((x |||  y) +  (x &&&  y)) := by
+  bv_automata_circuit
+
+
+def test15 (x y : BitVec w) : (x - y) = (( x &&& (~~~ y)) - ((~~~ x) &&&  y)) := by
+  bv_automata_circuit
+
+def test17 (x y : BitVec w) : (x ^^^ y) = ((x ||| y) - (x &&& y)) := by
+  bv_automata_circuit
+
+
+def test18 (x y : BitVec w) : (x &&&  (~~~ y)) = ((x ||| y) - y) := by
+  bv_automata_circuit
+
+
+def test19 (x y : BitVec w) : (x &&&  (~~~ y)) = (x -  (x &&& y)) := by
+  bv_automata_circuit
+
+
+def test21 (x y : BitVec w) : (~~~(x - y)) = (~~~x + y) := by
+  bv_automata_circuit
+
+def test2_circuit (x y : BitVec w) : (~~~(x ^^^ y)) = ((x &&& y) + ~~~(x ||| y)) := by
+  bv_automata_circuit
+
+def test24 (x y : BitVec w) : (x ||| y) = (( x &&& (~~~y)) + y) := by
+  bv_automata_circuit
+
+/--
+info: 'Reflect.test24' depends on axioms: [propext, Classical.choice, Lean.ofReduceBool, Lean.trustCompiler, Quot.sound]
+-/
+#guard_msgs in #print axioms test24
+
+/--
+info: def Reflect.test24 : ∀ {w : ℕ} (x y : BitVec w), x ||| y = (x &&& ~~~y) + y :=
+fun {w} x y =>
+  id
+    (Predicate.denote_of_eval_eq
+      (of_decide_eq_true
+        (ofReduceBool
+          (decide
+            (∀ (w : ℕ) (vars : List BitStream),
+              (Predicate.binary BinaryPredicate.eq ((Term.var 0).or (Term.var 1))
+                      (((Term.var 0).and (Term.var 1).not).add (Term.var 1))).eval
+                  vars w =
+                false))
+          true SSA.Experimental.Bits.Fast.Reflect._auxLemma.32))
+      w (Map.append w y (Map.append w x Map.empty)))
+-/
+#guard_msgs in #print test24
+
+def test25 (x y : BitVec w) : (x &&& y) = (((~~~x) ||| y) - ~~~x) := by
+  bv_automata_circuit
+
+def test26 {w : Nat} (x y : BitVec w) : 1#w + x + 0#w = 1#w + x := by
+  bv_automata_circuit
+
+/-- NOTE: we now support 'ofNat' literals -/
+def test27 (x y : BitVec w) : 2#w + x  = 1#w  + x + 1#w := by
+  bv_automata_circuit
+
+def test28 {w : Nat} (x y : BitVec w) : x &&& x &&& x &&& x &&& x &&& x = x := by
+  bv_automata_circuit
+
+example : ∀ (w : Nat) , (BitVec.ofNat w 1) &&& (BitVec.ofNat w 3) = BitVec.ofNat w 1 := by
+  intros
+  bv_automata_circuit
+
+example : ∀ (w : Nat) (x : BitVec w), -1#w &&& x = x := by
+  intros
+  bv_automata_circuit
+
+example : ∀ (w : Nat) (x : BitVec w), x <<< (0 : Nat) = x := by intros; bv_automata_circuit
+example : ∀ (w : Nat) (x : BitVec w), x <<< (1 : Nat) = x + x := by intros; bv_automata_circuit
+example : ∀ (w : Nat) (x : BitVec w), x <<< (2 : Nat) = x + x + x + x := by
+  intros w n
+  -- rw [BitVec.ofNat_eq_ofNat (n := w) (i := 2)]
+  intros; bv_automata_circuit
+
+/-- Can solve width-constraints problems -/
+def test30  : (w = 2) → 8#w = 0#w := by
+  bv_automata_circuit
+
+/-- Can solve width-constraints problems -/
+def test31 (w : Nat) (x : BitVec w) : x &&& x = x := by
+  bv_automata_circuit (config := { stateSpaceSizeThreshold := 100 })
+
+theorem neg_eq_not_add_one (x : BitVec w) :
+    -x = ~~~ x + 1#w := by
+  bv_automata_circuit
+
+theorem add_eq_xor_add_mul_and (x y : BitVec w) :
+    x + y = (x ^^^ y) + (x &&& y) + (x &&& y) := by
+  bv_automata_circuit (config := { circuitSizeThreshold := 300 } )
+
+theorem add_eq_xor_add_mul_and' (x y : BitVec w) :
+    x + y = (x ^^^ y) + (x &&& y) + (x &&& y) := by
+  bv_automata_circuit (config := { circuitSizeThreshold := 300 } )
+
+theorem add_eq_xor_add_mul_and_nt (x y : BitVec w) :
+    x + y = (x ^^^ y) + 2 * (x &&& y) := by
+  bv_automata_circuit
+
+/-- Check that we correctly process an even numeral multiplication. -/
+theorem mul_four (x : BitVec w) : 4 * x = x + x + x + x := by
+  bv_automata_circuit
+
+/-- Check that we correctly process an odd numeral multiplication. -/
+theorem mul_five (x : BitVec w) : 5 * x = x + x + x + x + x := by
+  bv_automata_circuit (config := { circuitSizeThreshold := 180 })
+
+open BitVec in
+/-- Check that we support sign extension. -/
+theorem sext
+    (b : BitVec 8)
+    (c : ¬(11#9 - signExtend 9 (b &&& 7#8)).msb = (11#9 - signExtend 9 (b &&& 7#8)).getMsbD 1) :
+    False := by
+  fail_if_success bv_automata_circuit
+  sorry
+
+/-- Check that we support zero extension. -/
+theorem zext (b : BitVec 8) : (b.zeroExtend 10 |>.zeroExtend 8) = b := by
+  fail_if_success bv_automata_circuit
+  sorry
+
+/-- Can solve width-constraints problems, when written with a width constraint. -/
+def width_specific_1 (x : BitVec w) : w = 1 →  x + x = x ^^^ x := by
+  bv_automata_circuit
+
+
+example (x : BitVec 0) : x = x + 0#0 := by
+  bv_automata_circuit
+
+/-- All bitvectors are equal at width 0 -/
+example (x y : BitVec w) (hw : w = 0) : x = y := by
+  bv_automata_circuit
+
+/-- At width 1, adding bitvector to itself four times gives 0. Characteristic equals 2 -/
+def width_1_char_2 (x : BitVec w) (hw : w = 1) : x + x = 0#w := by
+  bv_automata_circuit
+
+/-- At width 1, adding bitvector to itself four times gives 0. Characteristic 2 divides 4 -/
+def width_1_char_2_add_four (x : BitVec w) (hw : w = 1) : x + x + x + x = 0#w := by
+  bv_automata_circuit
+
+/--
+info: 'Reflect.width_1_char_2_add_four' depends on axioms: [propext,
+ Classical.choice,
+ Lean.ofReduceBool,
+ Lean.trustCompiler,
+ Quot.sound]
+-/
+#guard_msgs in #print axioms width_1_char_2_add_four
+
+set_option trace.profiler true  in
+/-- warning: declaration uses 'sorry' -/
+theorem slow₁ (x : BitVec 32) :
+    63#32 - (x &&& 31#32) = x &&& 31#32 ^^^ 63#32 := by
+  fail_if_success bv_automata_circuit (config := { circuitSizeThreshold := 30, stateSpaceSizeThreshold := 24 } )
+  sorry
+
+theorem neg_one_mul (x y : BitVec w) :
+     - 1 *  ~~~(x ^^^ y)  = -1 * ~~~ (x ^^^ y) := by
+  bv_automata_circuit
+
+theorem e_1 (x y : BitVec w) :
+     - 1 *  ~~~(x ^^^ y) - 2 * y + 1 *  ~~~x =  - 1 *  ~~~(x |||  ~~~y) - 3 * (x &&& y) := by
+  bv_automata_circuit (config := { backend := .cadical })
+
+end BvAutomataTests
 
 end Reflect
